[DSL] add sound instance generation

Veil/DSL/ActionTheory.lean
@@ -124,6 +124,14 @@ def Wlp.spec (req : SProp σ) (ens : σ -> RProp σ ρ) : Wlp m σ ρ :=
 def BigStep.spec (req : SProp σ) (ens : σ -> RProp σ ρ) : BigStep σ ρ :=
   fun s r s' => req s -> ens s r s'
 
+@[actSimp]
+def Wlp.get : Wlp m σ σ := fun s post => post s s
+@[actSimp]
+def Wlp.set (s' : σ) : Wlp m σ Unit := fun _ post => post () s'
+@[actSimp]
+def Wlp.modifyGet (act : σ -> ρ × σ) : Wlp m σ ρ := fun s post => let (ret, s') := act s ; post ret s'
+
+
 -- def BigStep.choice : BigStep σ ρ -> BigStep σ ρ -> BigStep σ ρ :=
 --   fun act act' s r s' => act s r s' ∨ act' s r s'
 
@@ -141,17 +149,36 @@ instance : Monad (Wlp m σ) where
   bind := Wlp.bind
 
 instance : MonadStateOf σ (Wlp m σ) where
-  get := fun s post => post s s
-  set s' := fun _ post => post () s'
-  modifyGet := fun act s post => let (ret, s') := act s ; post ret s'
+  get := Wlp.get
+  set := Wlp.set
+  modifyGet := Wlp.modifyGet
+
+@[wlpSimp]
+def pureE : pure = Wlp.pure (σ := σ) (ρ := ρ) (m := m) := rfl
+@[wlpSimp]
+def bindE : bind = Wlp.bind (σ := σ) (ρ := ρ) (ρ' := ρ') (m := m) := rfl
+@[wlpSimp]
+def getE : get = Wlp.get (σ := σ) (m := m) := rfl
+@[wlpSimp]
+def modifyGetE : modifyGet = Wlp.modifyGet (σ := σ) (ρ := ρ) (m := m) := rfl
+
 
 class IsStateExtension (σ : semiOutParam Type) (σ' : Type) where
   extendWith : σ -> σ' -> σ'
   restrictTo : σ' -> σ
 
 export IsStateExtension (extendWith restrictTo)
+
+@[actSimp]
+def Wlp.lift {σ σ'} [IsStateExtension σ σ'] (act : Wlp m σ ρ) : Wlp m σ' ρ :=
+  fun s' post => act (restrictTo s') (fun r s => post r (extendWith s s'))
+
 instance [IsStateExtension σ σ'] : MonadLift (Wlp m σ) (Wlp m σ') where
-  monadLift := fun m s post => m (restrictTo s) (fun r s' => post r (extendWith s' s))
+  monadLift := Wlp.lift
+
+@[wlpSimp]
+def monadLiftE [IsStateExtension σ σ'] : monadLift = Wlp.lift (σ := σ) (σ' := σ') (ρ := ρ) (m := m) := rfl
+
 
 /-! ### Soundness proof -/
 
@@ -184,15 +211,15 @@ abbrev ActProp.triple {σ } (req : SProp σ) (act : ActProp σ) (ens : SProp σ)
   - third condition `call`, states that the `internal` mode of `act` refines the `external`
     one. In other words, if you have proven some striple for `internal` mode of `act`,
     the same one holds for its `external` version -/
-class Sound {σ ρ : Type} (act : (m : Mode) -> Wlp m σ ρ) where
-  inter {m} {τ : Type} [Inhabited τ] (post : τ -> RProp σ ρ) :
-    ∀ s : σ, (∀ t : τ, act m s (post t)) -> act m s (∀ t, post t · ·)
+class Sound {σ ρ : Type} (act : Wlp m σ ρ) where
+  inter {τ : Type} [Inhabited τ] (post : τ -> RProp σ ρ) :
+    ∀ s : σ, (∀ t : τ, act s (post t)) -> act s (∀ t, post t · ·)
   impl (post post' : RProp σ ρ) : ∀ s,
-    (∀ r s, post r s -> post' r s) -> act m s post -> act m s post'
-  call : act .internal <= act .external
+    (∀ r s, post r s -> post' r s) -> act s post -> act s post'
+  -- call : act .internal <= act .external
 
-theorem sound_and (act : ∀ m, Wlp m σ ρ) [Sound act] :
-  act m s post -> act m s post' -> act m s fun r s => post r s ∧ post' r s := by
+theorem sound_and (act : Wlp m σ ρ) [Sound act] :
+  act s post -> act s post' -> act s fun r s => post r s ∧ post' r s := by
   intro hact hact'
   let Post := fun (b : Bool) => if b then post' else post
   have post_eq : (fun r s => ∀ b, Post b r s) = fun r s => post r s ∧ post' r s := by
@@ -228,7 +255,7 @@ theorem sound_and (act : ∀ m, Wlp m σ ρ) [Sound act] :
 
 theorem triple_sound [Sound act] (req : SProp σ) (ens : SProp σ) :
   (¬ ∀ s, ens s) ->
-  (act m).toActProp.triple req ens -> (act m).triple req (fun _ => ens) := by
+  act.toActProp.triple req ens -> act.triple req (fun _ => ens) := by
   intro ensTaut htriple s hreq
   have ens_impl : ∀ s, (∀ s' : { s' // ¬ ens s' }, ¬ (s'.val = s)) -> ens s := by
     simp; intro s impl
@@ -242,94 +269,100 @@ theorem triple_sound [Sound act] (req : SProp σ) (ens : SProp σ) :
   false_or_by_contra
   specialize htriple _ _ ‹_› ‹_›; contradiction
 
-instance : Sound (Wlp.pure (m := ·) (σ := σ) r) where
-  inter := by simp [actSimp]
-  impl  := by intros; simp_all [actSimp]
-  call  := by solve_by_elim
+instance pure_sound : Sound (Wlp.pure (σ := σ) (m := m) r) where
+  inter := by simp [pure, actSimp]
+  impl  := by intros; simp_all [pure, actSimp]
+  -- call  := by solve_by_elim
 
-instance (act' : ρ -> ∀ m, Wlp m σ ρ) [Sound act] [∀ r, Sound (act' r)] : Sound (fun m => Wlp.bind (act m) (act' · m)) where
+instance bind_sound (act' : ρ -> Wlp m σ ρ') [Sound act] [∀ r, Sound (act' r)] : Sound (Wlp.bind act act') where
   inter := by
     unfold Wlp.bind
-    intros m τ _ post s hbind
-    apply Sound.impl (∀ t, act' · m · <| post t) <;> solve_by_elim [Sound.inter]
+    intros τ _ post s hbind
+    apply Sound.impl (∀ t, act' · · <| post t) <;> solve_by_elim [Sound.inter]
   impl := by
     unfold Wlp.bind
-    intros m post post' s hpost hbind
-    apply Sound.impl (act' · m · <| post) <;> (intros; solve_by_elim [Sound.impl])
-  call := by
-    unfold Wlp.bind
-    intros s post hbind
-    apply Sound.call; apply Sound.impl;
-    { intros _ _; apply Sound.call }
-    solve_by_elim
+    intros post post' s hpost hbind
+    apply Sound.impl (act' · · <| post) <;> (intros; solve_by_elim [Sound.impl])
+  -- call := by
+  --   unfold Wlp.bind
+  --   intros s post hbind
+  --   apply Sound.call; apply Sound.impl;
+  --   { intros _ _; apply Sound.call }
+  --   solve_by_elim
 
-instance : Sound (Wlp.assume (m := ·) (σ := σ) rq) where
+instance assume_sound : Sound (Wlp.assume (m := m) (σ := σ) rq) where
   inter := by intros; simp_all [actSimp]
   impl := by intros; simp_all [actSimp]
-  call := by solve_by_elim
+  -- call := by solve_by_elim
 
-instance : Sound (Wlp.assert (m := ·) (σ := σ) rq) where
+instance assert_sound : Sound (Wlp.assert (m := m) (σ := σ) rq) where
   inter := by intros; simp_all [actSimp]; rename_i h; specialize h default; simp [*]
   impl  := by intros; simp_all [actSimp] <;> solve_by_elim
-  call  := by solve_by_elim
+  -- call  := by solve_by_elim
 
-instance : Sound (Wlp.require (m := ·) (σ := σ) rq) where
+instance require_sound : Sound (Wlp.require (m := m) (σ := σ) rq) where
   inter := by
-    intros m; cases m
+    cases m
     { intros; simp_all [actSimp]; rename_i h; specialize h default; simp [*] }
     intros; simp_all [actSimp]
-  impl := by intros m; cases m <;> (intros; simp_all [actSimp] <;> solve_by_elim)
-  call := by
-   intros s post; unfold Wlp.require; simp [Wlp.assert, Wlp.assume]; solve_by_elim
+  impl := by cases m <;> (intros; simp_all [actSimp] <;> solve_by_elim)
+  -- call := by
+  --  intros s post; unfold Wlp.require; simp [Wlp.assert, Wlp.assume]; solve_by_elim
 
 
-instance : Sound (Wlp.fresh (m := ·) (σ := σ) τ) where
+instance fresh_sound : Sound (Wlp.fresh (m := m) (σ := σ) τ) where
   inter := by intros; simp_all [actSimp]
   impl := by intros; simp_all [actSimp]
-  call := by solve_by_elim
+  -- call := by solve_by_elim
 
 
-instance : Sound (Wlp.spec (m := ·) req ens) where
+instance spec_sound : Sound (Wlp.spec (m := m) req ens) where
   inter := by
-    intro m; cases m <;> (intros; simp_all [actSimp])
+    cases m <;> (intros; simp_all [actSimp])
     rename_i h; intros; specialize h default; simp [*]
   impl := by
-    intro m; cases m <;> (simp [actSimp]; intros)
+    cases m <;> (simp [actSimp]; intros)
     { constructor <;> (intros; solve_by_elim) }
     solve_by_elim
-  call := by intros _; simp_all [actSimp]
+  -- call := by intros _; simp_all [actSimp]
 
-instance (r : σ -> σ -> Prop) : Sound (r.toWlp (m := ·)) where
+instance (r : σ -> σ -> Prop) : Sound (r.toWlp (m := m)) where
   inter := by intros; simp_all [actSimp]
   impl := by intros; simp_all [actSimp]
-  call := by solve_by_elim
+  -- call := by solve_by_elim
 
-instance : Sound (get (m := Wlp · σ)) where
-  inter := by intros; simp_all [get, getThe,MonadStateOf.get]
-  impl := by intros; simp_all [get, getThe,MonadStateOf.get]
-  call := by solve_by_elim
+instance get_sound : Sound (Wlp.get (m := m) (σ := σ)) where
+  inter := by intros; simp_all [get, getThe,MonadStateOf.get, Wlp.get]
+  impl := by intros; simp_all [get, getThe,MonadStateOf.get,Wlp.get]
+  -- call := by solve_by_elim
 
-instance (s : σ) : Sound (set s (m := Wlp · σ)) where
-  inter := by intros; simp_all [set,MonadStateOf.set]
-  impl := by intros; simp_all [set,MonadStateOf.set]
-  call := by solve_by_elim
+instance set_sound (s : σ) : Sound (Wlp.set s (m := m)) where
+  inter := by intros; simp_all [Wlp.set]
+  impl := by intros; simp_all [Wlp.set]
+  -- call := by solve_by_elim
 
-instance : Sound (modifyGet f (m := Wlp · σ)) where
-  inter := by intros; simp_all [modifyGet,MonadStateOf.modifyGet]
-  impl := by intros; simp_all [modifyGet,MonadStateOf.modifyGet]
-  call := by solve_by_elim
+instance modifyGet_sound : Sound (Wlp.modifyGet f (m := m) (σ := σ) (ρ := ρ)) where
+  inter := by intros; simp_all [Wlp.modifyGet]
+  impl := by intros; simp_all [Wlp.modifyGet]
+  -- call := by solve_by_elim
 
-instance (act : ∀ m, Wlp m σ ρ) [IsStateExtension σ σ'] [Sound act] :
-  Sound (fun m => monadLift (m := Wlp m σ) (n := Wlp m σ') (act m)) where
+instance if_sound [Decidable c] [instT: Sound t] [instS : Sound e] : Sound (ite c t e) where
   inter := by
-    intros; simp_all [monadLift, MonadLift.monadLift]
+    intros; by_cases c <;> simp_all <;> solve_by_elim [instT.inter, instS.inter]
+  impl := by
+    intros; by_cases c <;> simp_all <;> solve_by_elim [instT.impl, instS.impl]
+
+instance (act : Wlp m σ ρ) [IsStateExtension σ σ'] [Sound act] :
+  Sound (act.lift (σ' := σ')) where
+  inter := by
+    intros; simp_all [Wlp.lift]
     solve_by_elim [Sound.inter]
   impl := by
-    intros; simp_all [monadLift, MonadLift.monadLift]
+    intros; simp_all [Wlp.lift]
     solve_by_elim [Sound.impl]
-  call := by
-    intros; simp_all [monadLift, MonadLift.monadLift]
-    solve_by_elim [Sound.call]
+  -- call := by
+  --   intros; simp_all [monadLift, MonadLift.monadLift]
+  --   solve_by_elim [Sound.call]
 
 /-! ### Correctness of `checkSpec` -/
 
@@ -338,8 +371,8 @@ theorem wlp_spec_to_big_step :
   ext s r' s'; unfold Wlp.spec BigStep.spec Wlp.toBigStep; simp
 
 theorem check_spec_sound [Sound act] (req : SProp σ) (ens : σ -> RProp σ ρ) :
-  (∀ s, req s -> act m s (ens s)) ->
-  Wlp.spec (m := .internal) req ens <= act m := by
+  (∀ s, req s -> act s (ens s)) ->
+  Wlp.spec (m := .internal) req ens <= act := by
   intro triple s post; simp [actSimp]; intros hreq hens
   solve_by_elim [Sound.impl]
 
