Veil/DSL/Base.lean
@@ -4,6 +4,7 @@ open Lean
 register_simp_attr invSimp
 register_simp_attr ifSimp
 register_simp_attr actSimp
+register_simp_attr wlpSimp
 register_simp_attr initSimp
 register_simp_attr safeSimp
 register_simp_attr genSimp
@@ -14,3 +15,8 @@ initialize
   registerTraceClass `dsl.info
   -- the following are primarily for performance profiling
   registerTraceClass `dsl.perf.checkInvariants
+
+register_option veil.gen_sound : Bool := {
+  defValue := false
+  descr := "generate soundness instances for actions"
+}
